{
  "nbformat": 4,
  "nbformat_minor": 0,
  "metadata": {
    "colab": {
      "provenance": []
    },
    "kernelspec": {
      "name": "python3",
      "display_name": "Python 3"
    },
    "language_info": {
      "name": "python"
    }
  },
  "cells": [
    {
      "cell_type": "markdown",
      "source": [
        "### Conic Sections: Key Concepts and Formulas\n",
        "\n",
        "Conic sections refer to the curves obtained by intersecting a plane with a cone. The basic types of conic sections are the **circle**, **ellipse**, **parabola**, and **hyperbola**. These curves are defined by specific equations, and understanding how to derive and manipulate these equations is crucial in geometry and calculus.\n",
        "\n",
        "---\n",
        "\n",
        "#### **Circle**\n",
        "A **circle** is the set of all points in a plane that are equidistant from a fixed point, called the center.\n",
        "\n",
        "- **Standard Equation of a Circle:**\n",
        "  The standard equation of a circle with center \\((h, k)\\) and radius \\(r\\) is:  \n",
        "  $$ (x - h)^2 + (y - k)^2 = r^2 $$\n",
        "\n",
        "---\n",
        "\n",
        "#### **Parabola**\n",
        "A **parabola** is the set of all points equidistant from a fixed point, called the focus, and a fixed line, called the directrix.\n",
        "\n",
        "- **Standard Equation of a Parabola:**\n",
        "  The standard equation of a parabola opening vertically (up or down) is:  \n",
        "  $$ y - k = a(x - h)^2 $$  \n",
        "  The standard equation of a parabola opening horizontally (left or right) is:  \n",
        "  $$ x - h = a(y - k)^2 $$  \n",
        "  Where \\((h, k)\\) is the vertex and \\(a\\) is a constant that affects the width of the parabola.\n",
        "\n",
        "---\n",
        "\n",
        "#### **Ellipse**\n",
        "An **ellipse** is the set of all points for which the sum of the distances to two fixed points, called foci, is constant.\n",
        "\n",
        "- **Standard Equation of an Ellipse:**\n",
        "  The standard equation of an ellipse centered at the origin is:  \n",
        "  $$ \\frac{x^2}{a^2} + \\frac{y^2}{b^2} = 1 $$  \n",
        "  Where \\(a\\) is the length of the semi-major axis and \\(b\\) is the length of the semi-minor axis.  \n",
        "  If the center is at \\((h, k)\\), the equation becomes:  \n",
        "  $$ \\frac{(x - h)^2}{a^2} + \\frac{(y - k)^2}{b^2} = 1 $$\n",
        "\n",
        "---\n",
        "\n",
        "#### **Hyperbola**\n",
        "A **hyperbola** is the set of all points where the absolute difference of the distances to two fixed points (the foci) is constant.\n",
        "\n",
        "- **Standard Equation of a Hyperbola:**\n",
        "  The standard equation of a hyperbola centered at the origin is:  \n",
        "  $$ \\frac{x^2}{a^2} - \\frac{y^2}{b^2} = 1 $$  \n",
        "  Where \\(a\\) is the distance from the center to each vertex, and \\(b\\) is related to the asymptotes.  \n",
        "  If the center is at \\((h, k)\\), the equation becomes:  \n",
        "  $$ \\frac{(x - h)^2}{a^2} - \\frac{(y - k)^2}{b^2} = 1 $$\n",
        "\n",
        "---\n",
        "\n",
        "#### **Tangents to Conic Sections**\n",
        "The tangent line to a conic section at a given point is the line that touches the curve at that point without crossing it.\n",
        "\n",
        "- **Equation of the Tangent to a Circle:**\n",
        "  The equation of the tangent to a circle \\( (x - h)^2 + (y - k)^2 = r^2 \\) at the point \\((x_1, y_1)\\) on the circle is:  \n",
        "  $$ (x_1 - h)(x - h) + (y_1 - k)(y - k) = r^2 $$\n",
        "\n",
        "---\n"
      ],
      "metadata": {
        "id": "-1s4zuSc_vX2"
      }
    },
    {
      "cell_type": "markdown",
      "source": [
        "## Tasks related to conic sections\n",
        "\n",
        "**Visualize each task.** - Python, GeoGebra, Wolfram Alpha, ...\n",
        "\n",
        "* Find the equation of a circle with center at point $A(1,2)$ and radius $r=3$.\n",
        "* Find the equation of a parabola intersecting the $Ox$ axis at points $x=2$, $x=4$, and passing through point $y(3)=1$.\n",
        "* Find the center of the ellipse with the equation $x^2 + 4y^2 - 4x - 16y + 16 = 0$.\n",
        "* Find the slope ($m>0$) of the line $y=mx-5$ that is tangent to the circle with the equation $x^2 + y^2=1$.\n",
        "* Find the intersection points of the hyperbola $x^2 - y^2 = 1$ with the ellipse's line $x^2 + 4y^2 = 6$.\n",
        "* For the given hyperbola $x^2 - y^2 = 1$, find the distance between its branches."
      ],
      "metadata": {
        "id": "eXgpOWCS_2jt"
      }
    },
    {
      "cell_type": "markdown",
      "source": [
        "$$Q 1$$\n",
        "\n",
        "### Find the equation of a circle with center at point \\( A(1,2) \\) and radius \\( r = 3 \\)\n",
        "\n",
        "The general equation of a circle with center \\( (h, k) \\) and radius \\( r \\) is:\n",
        "\n",
        "$$ (x - h)^2 + (y - k)^2 = r^2 $$\n",
        "\n",
        "Given:\n",
        "- Center \\( A(1, 2) \\), so \\( h = 1 \\) and \\( k = 2 \\).\n",
        "- Radius \\( r = 3 \\).\n",
        "\n",
        "Substituting these values into the equation:\n",
        "\n",
        "$$ (x - 1)^2 + (y - 2)^2 = 3^2 $$  \n",
        "$$ (x - 1)^2 + (y - 2)^2 = 9 $$\n",
        "\n",
        "Thus, the equation of the circle is:\n",
        "\n",
        "$$ (x - 1)^2 + (y - 2)^2 = 9 $$\n"
      ],
      "metadata": {
        "id": "ehnrLBRoCL7i"
      }
    },
    {
      "cell_type": "markdown",
      "source": [
        "$$Q 2$$\n",
        "\n",
        "### Find the equation of a parabola intersecting the \\( Ox \\) axis at points \\( x = 2 \\), \\( x = 4 \\), and passing through point \\( y(3) = 1 \\)\n",
        "\n",
        "The general form of the equation of a parabola is:\n",
        "\n",
        "$$ y = a(x - h)^2 + k $$\n",
        "\n",
        "Given that the parabola intersects the \\( Ox \\) axis at \\( x = 2 \\) and \\( x = 4 \\), the equation can be written as:\n",
        "\n",
        "$$ y = a(x - 2)(x - 4) $$\n",
        "\n",
        "We use the point \\( (3, 1) \\) to find the value of \\( a \\):\n",
        "\n",
        "Substitute \\( x = 3 \\) and \\( y = 1 \\):\n",
        "\n",
        "$$ 1 = a(3 - 2)(3 - 4) $$  \n",
        "$$ 1 = a(1)(-1) $$  \n",
        "$$ 1 = -a $$  \n",
        "Thus, \\( a = -1 \\).\n",
        "\n",
        "Therefore, the equation of the parabola is:\n",
        "\n",
        "$$ y = -(x - 2)(x - 4) $$\n",
        "\n",
        "Expanding:\n",
        "\n",
        "$$ y = -x^2 + 6x - 8 $$\n",
        "\n",
        "Thus, the equation of the parabola is:\n",
        "\n",
        "$$ y = -x^2 + 6x - 8 $$\n"
      ],
      "metadata": {
        "id": "AuGDm6WMChz1"
      }
    },
    {
      "cell_type": "markdown",
      "source": [
        "$$Q 3$$\n",
        "\n",
        "### Find the center of the ellipse with the equation \\( x^2 + 4y^2 - 4x - 16y + 16 = 0 \\)\n",
        "\n",
        "We complete the square for both \\( x \\) and \\( y \\):\n",
        "\n",
        "The given equation is:\n",
        "\n",
        "$$ x^2 + 4y^2 - 4x - 16y + 16 = 0 $$\n",
        "\n",
        "Group the \\( x \\)-terms and \\( y \\)-terms:\n",
        "\n",
        "$$ (x^2 - 4x) + 4(y^2 - 4y) + 16 = 0 $$\n",
        "\n",
        "___\n",
        "### Complete the square:\n",
        "\n",
        "- For \\( x^2 - 4x \\), add and subtract \\( 4 \\):\n",
        "\n",
        "$$ x^2 - 4x = (x^2 - 4x + 4) - 4 = (x - 2)^2 - 4 $$\n",
        "\n",
        "- For \\( y^2 - 4y \\), factor out \\( 4 \\), then complete the square for \\( y^2 - 4y \\) (add \\( 4 \\)):\n",
        "\n",
        "$$ y^2 - 4y = 4\\left(y^2 - y\\right) $$\n",
        "\n",
        "Now, complete the square inside the parentheses:\n",
        "\n",
        "$$ y^2 - y = (y - \\frac{1}{2})^2 - \\frac{1}{4} $$\n",
        "\n",
        "Thus, we have:\n",
        "\n",
        "$$ 4\\left(y^2 - y\\right) = 4\\left( (y - \\frac{1}{2})^2 - \\frac{1}{4} \\right) = 4(y - \\frac{1}{2})^2 - 1 $$\n",
        "\n",
        "\n",
        "Thus:\n",
        "\n",
        "$$ (x^2 - 4x + 4) + 4(y^2 - 4y + 4) + 16 - 4 - 16 = 0 $$  \n",
        "$$ (x - 2)^2 + 4(y - 2)^2 = 4 $$\n",
        "\n",
        "Now divide by 4:\n",
        "\n",
        "$$ \\frac{(x - 2)^2}{4} + \\frac{(y - 2)^2}{1} = 1 $$\n",
        "\n",
        "The center of the ellipse is at \\( (2, 2) \\).\n"
      ],
      "metadata": {
        "id": "RsitoCBzCm1L"
      }
    },
    {
      "cell_type": "markdown",
      "source": [
        "$$Q 4$$\n",
        "\n",
        "The distance from a point \\( (x_1, y_1) \\) to a line \\( Ax + By + C = 0 \\) is given by:\n",
        "\n",
        "$$ d = \\frac{|Ax_1 + By_1 + C|}{\\sqrt{A^2 + B^2}} $$\n",
        "\n",
        "For the line \\( y = mx - 5 \\), we rewrite it as:\n",
        "\n",
        "$$ mx - y - 5 = 0 $$\n",
        "\n",
        "The center of the circle is at \\( (0, 0) \\). Thus, the distance from the center to the line is:\n",
        "\n",
        "$$ d = \\frac{|m(0) - 1(0) - 5|}{\\sqrt{m^2 + 1}} $$  \n",
        "$$ d = \\frac{| - 5 |}{\\sqrt{m^2 + 1}} $$  \n",
        "$$ d = \\frac{5}{\\sqrt{m^2 + 1}} $$\n",
        "\n",
        "For tangency, the distance must equal the radius (1):\n",
        "\n",
        "$$ \\frac{5}{\\sqrt{m^2 + 1}} = 1 $$\n",
        "\n",
        "Solve for \\( m \\):\n",
        "\n",
        "$$ 5 = \\sqrt{m^2 + 1} $$  \n",
        "$$ 25 = m^2 + 1 $$  \n",
        "$$ m^2 = 24 $$  \n",
        "$$ m = \\sqrt{24} $$  \n",
        "$$ m = 2\\sqrt{6} $$\n",
        "\n"
      ],
      "metadata": {
        "id": "frPbfPZaDJot"
      }
    },
    {
      "cell_type": "markdown",
      "source": [
        "$$Q 5$$\n",
        "\n",
        "### Find the intersection points of the hyperbola \\( x^2 - y^2 = 1 \\) with the ellipse's line \\( x^2 + 4y^2 = 6 \\)\n",
        "\n",
        "We solve the system of equations:\n",
        "\n",
        "$$ 1. \\quad x^2 - y^2 = 1 $$  \n",
        "$$ 2. \\quad x^2 + 4y^2 = 6 $$\n",
        "\n",
        "From the first equation, solve for \\( x^2 \\):\n",
        "\n",
        "$$ x^2 = y^2 + 1 $$\n",
        "\n",
        "Substitute into the second equation:\n",
        "\n",
        "$$ (y^2 + 1) + 4y^2 = 6 $$  \n",
        "$$ y^2 + 1 + 4y^2 = 6 $$  \n",
        "$$ 5y^2 + 1 = 6 $$  \n",
        "$$ 5y^2 = 5 $$  \n",
        "$$ y^2 = 1 $$  \n",
        "$$ y = \\pm 1 $$\n",
        "\n",
        "Substitute \\( y = 1 \\) and \\( y = -1 \\) into \\( x^2 = y^2 + 1 \\):\n",
        "\n",
        "For \\( y = 1 \\):  \n",
        "$$ x^2 = 1 + 1 = 2 $$  \n",
        "$$ x = \\pm \\sqrt{2} $$\n",
        "\n",
        "For \\( y = -1 \\):  \n",
        "$$ x^2 = 1 + 1 = 2 $$  \n",
        "$$ x = \\pm \\sqrt{2} $$\n",
        "\n",
        "Thus, the intersection points are $$ (\\sqrt{2}, 1) $$, $$ (-\\sqrt{2}, 1) $$, $$ (\\sqrt{2}, -1) $$, and $$ (-\\sqrt{2}, -1) $$.\n"
      ],
      "metadata": {
        "id": "3JmuD-wHDTPT"
      }
    },
    {
      "cell_type": "markdown",
      "source": [
        "$$Q 6$$\n",
        "\n",
        "### For the given hyperbola \\( x^2 - y^2 = 1 \\), find the distance between its branches\n",
        "\n",
        "\n",
        "For the equation \\( x^2 - y^2 = 1 \\), we compare it with the standard form:\n",
        "\n",
        "$$ \\frac{x^2}{1} - \\frac{y^2}{1} = 1 $$\n",
        "\n",
        "Here, \\( a^2 = 1 \\) and \\( b^2 = 1 \\), so \\( b = 1 \\).\n",
        "\n",
        "Thus, the distance between the branches is:\n",
        "\n",
        "$$ 2b = 2 \\times 1 = 2 $$\n"
      ],
      "metadata": {
        "id": "fBELgfmMEfls"
      }
    }
  ]
}